doubly-linked list lru implementation

lib/LRU.i.dfy
@@ -2,6 +2,7 @@
 
 include "NativeTypes.s.dfy"
 include "Sequences.s.dfy"
+include "MutableMap.i.dfy"
 
 module LruModel {
 	export S provides LruQueue, WF, I, Empty, Remove, Use, Pop, Next, LruUse, LruRemove, NativeTypes
@@ -28,7 +29,7 @@ module LruModel {
 
   function I(q: LruQueue) : set<uint64>
   {
-    set i | i in q
+    set x | x in q
   }
 
   function method Empty() : (q : LruQueue)
@@ -39,21 +40,21 @@ module LruModel {
     []
   }
 
-  function method Remove(q: LruQueue, i: uint64) : LruQueue
+  function method Remove(q: LruQueue, x: uint64) : LruQueue
   {
     if |q| == 0 then [] else (
-      if Last(q) == i then Remove(DropLast(q), i) else Remove(DropLast(q), i) + [Last(q)]
+      if Last(q) == x then Remove(DropLast(q), x) else Remove(DropLast(q), x) + [Last(q)]
     )
   }
 
-  function method Use(q: LruQueue, i: uint64) : LruQueue
+  function method Use(q: LruQueue, x: uint64) : LruQueue
   {
-    Remove(q, i) + [i]
+    Remove(q, x) + [x]
   }
 
-  function method Next(q: LruQueue) : (i : uint64)
+  function method Next(q: LruQueue) : (x : uint64)
   requires |I(q)| > 0
-  ensures i in I(q)
+  ensures x in I(q)
   {
     q[0]
   }
@@ -64,13 +65,342 @@ module LruModel {
     (q[1..], q[0])
   }
 
-  lemma LruUse(q: LruQueue, i: uint64)
+  lemma LruUse(q: LruQueue, x: uint64)
   requires WF(q)
-  ensures WF(Use(q, i))
-  ensures I(Use(q, i)) == I(q) + {i}
+  ensures WF(Use(q, x))
+  ensures I(Use(q, x)) == I(q) + {x}
 
-  lemma LruRemove(q: LruQueue, i: uint64)
+  lemma LruRemove(q: LruQueue, x: uint64)
   requires WF(q)
-  ensures WF(Remove(q, i))
-  ensures I(Remove(q, i)) == I(q) - {i}
+  ensures WF(Remove(q, x))
+  ensures I(Remove(q, x)) == I(q) - {x}
+}
+
+module Lru {
+  import opened NativeTypes
+  import opened Sequences
+  import opened LruModel`Internal
+  import MutableMap
+
+  lemma lemmaRemoveNonPresentKeyFromQueue(q: LruQueue, x: uint64)
+  requires x !in q
+  requires WF(q)
+  ensures LruModel.Remove(q, x) == q
+  {
+    if |q| == 0 {
+    } else {
+      lemmaRemoveNonPresentKeyFromQueue(q[..|q|-1], x);
+    }
+  }
+
+  lemma LemmaQueueCountEqInterpCount(q: LruQueue)
+  requires WF(q)
+  ensures |I(q)| == |q|
+  {
+    reveal_distinct();
+    if |q| == 0 {
+    } else {
+      LemmaQueueCountEqInterpCount(q[..|q| - 1]);
+      assert I(q) == I(q[..|q|-1]) + {q[|q|-1]};
+      assert |I(q)|
+          == |I(q[..|q|-1]) + {q[|q|-1]}|
+          == |I(q[..|q|-1])| + |{q[|q|-1]}|
+          == |q[..|q|-1]| + 1
+          == |q|;
+    }
+  }
+
+  lemma lemmaGetRemoveQueueIndex(q: LruQueue, x: uint64)
+  returns (j: int)
+  requires x in q
+  requires WF(q)
+  ensures 0 <= j < |q|
+  ensures q[j] == x
+  ensures LruModel.Remove(q, x) == q[..j] + q[j+1..]
+  {
+    assert |q| > 0;
+    if q[|q| - 1] == x {
+      j := |q| - 1;
+      reveal_distinct();
+      lemmaRemoveNonPresentKeyFromQueue(q[..|q|-1], x);
+    } else {
+      j := lemmaGetRemoveQueueIndex(q[..|q|-1], x);
+    }
+  }
+
+  class Node {
+    var prev: Node?;
+    var next: Node?;
+    var value: uint64;
+
+    constructor (p: Node?, n: Node?, v: uint64)
+    ensures prev == p
+    ensures next == n
+    ensures value == v
+    {
+      prev := p;
+      next := n;
+      value := v;
+    }
+  }
+
+  class MutableLruQueue {
+    ghost var Queue: LruQueue;
+    ghost var Repr: set<object>;
+
+    var nodemap: MutableMap.ResizingHashMap<Node>;
+    var head_node: Node?;
+    var tail_node: Node?;
+
+    protected predicate Inv()
+    reads this, Repr
+    {
+      && nodemap in Repr
+      && nodemap.Repr <= Repr
+      && Repr == {this} + nodemap.Repr + nodemap.Contents.Values
+      && (|Queue| == 0 ==> (
+        && head_node == null
+        && tail_node == null
+        && nodemap.Contents == map[]
+      ))
+      && (forall i | 0 <= i < |Queue| :: Queue[i] in nodemap.Contents)
+      && (forall ref | ref in nodemap.Contents :: ref in Queue)
+      && (forall ref | ref in nodemap.Contents :: nodemap.Contents[ref].value == ref)
+      && (|Queue| > 0 ==>
+        && head_node == nodemap.Contents[Queue[0]]
+        && tail_node == nodemap.Contents[Queue[|Queue| - 1]]
+        && nodemap.Contents[Queue[0]].prev == null
+        && nodemap.Contents[Queue[|Queue| - 1]].next == null
+      )
+      && (forall i | 0 <= i < |Queue| - 1 ::
+          nodemap.Contents[Queue[i]].next == nodemap.Contents[Queue[i+1]])
+      && (forall i | 0 <= i < |Queue| - 1 ::
+          nodemap.Contents[Queue[i]] == nodemap.Contents[Queue[i+1]].prev)
+      && nodemap.Inv()
+      && nodemap.Repr !! nodemap.Contents.Values
+      && WF(Queue)
+    }
+
+    constructor ()
+    ensures Inv()
+    ensures Queue == Empty()
+    {
+      var m := new MutableMap.ResizingHashMap<Node>(128);
+
+      nodemap := m;
+      head_node := null;
+      tail_node := null;
+
+      Queue := [];
+      Repr := {this} + m.Repr + m.Contents.Values;
+    }
+
+    method Remove(x: uint64)
+    requires Inv()
+    ensures Inv()
+    ensures Queue == LruModel.Remove(old(Queue), x)
+    ensures Repr <= old(Repr)
+    modifies this, this.Repr
+    {
+      ghost var oldContents := nodemap.Contents;
+      ghost var oldQueue := Queue;
+
+      var node := nodemap.Remove(x);
+      if node.Some? {
+        var prev := node.value.prev;
+        var next := node.value.next;
+
+        ghost var j := lemmaGetRemoveQueueIndex(Queue, x);
+        if (j > 0) {
+          assert oldContents[x].prev == oldContents[Queue[j-1]];
+        }
+        if (j < |Queue| - 1) {
+          assert oldContents[x].next == oldContents[Queue[j+1]];
+        }
+
+        if (prev == null) {
+          head_node := next;
+        } else {
+          prev.next := next;
+        }
+
+        if (next == null) {
+          tail_node := prev;
+        } else {
+          next.prev := prev;
+        }
+
+        Repr := {this} + nodemap.Repr + nodemap.Contents.Values;
+        Queue := LruModel.Remove(Queue, x);
+
+        forall k | 0 <= k < |Queue| ensures Queue[k] in nodemap.Contents
+        {
+          reveal_distinct();
+          if k < j {
+            assert oldQueue[k] == Queue[k];
+            assert oldQueue[k] in oldContents;
+            assert oldQueue[k] != x;
+            assert oldQueue[k] in nodemap.Contents;
+          } else {
+            assert oldQueue[k+1] == Queue[k];
+            assert oldQueue[k+1] in oldContents;
+            assert oldQueue[k+1] != x;
+            assert oldQueue[k+1] in nodemap.Contents;
+          }
+        }
+
+        forall ref | ref in nodemap.Contents ensures ref in Queue
+        {
+          assert ref in oldContents;
+          var k :| 0 <= k < |oldQueue| && oldQueue[k] == ref;
+          assert k != j;
+          if k < j {
+            assert Queue[k] == ref;
+          } else {
+            assert Queue[k-1] == ref;
+          }
+        }
+
+        forall k | 0 <= k < |Queue| - 1
+        ensures nodemap.Contents[Queue[k]] == nodemap.Contents[Queue[k+1]].prev
+        {
+          if k < j-1 {
+            assert nodemap.Contents[Queue[k]] == nodemap.Contents[Queue[k+1]].prev;
+          } else if k == j-1 {
+            assert nodemap.Contents[Queue[k]] == nodemap.Contents[Queue[k+1]].prev;
+          } else {
+            assert nodemap.Contents[Queue[k]] == nodemap.Contents[Queue[k+1]].prev;
+          }
+        }
+      } else {
+        assert nodemap.Contents == oldContents;
+        lemmaRemoveNonPresentKeyFromQueue(Queue, x);
+
+        forall k | 0 <= k < |Queue| - 1
+        ensures nodemap.Contents[Queue[k]] == nodemap.Contents[Queue[k+1]].prev
+        {
+        }
+      }
+
+      LruRemove(oldQueue, x);
+    }
+
+    lemma LemmaMapCountEqInterpCount()
+    requires Inv()
+    ensures |I(Queue)| == nodemap.Count as int
+    {
+      assert I(Queue) == nodemap.Contents.Keys;
+      assert |I(Queue)|
+          == |nodemap.Contents.Keys|
+          ==|nodemap.Contents|
+          == nodemap.Count as int;
+    }
+
+    method Use(x: uint64)
+    requires Inv()
+    requires |I(Queue)| <= 0x10000
+    ensures Inv()
+    ensures Queue == LruModel.Use(old(Queue), x)
+    ensures forall x | x in Repr :: x in old(Repr) || fresh(x)
+    modifies this, this.Repr
+    {
+      ghost var oldContents := nodemap.Contents;
+      ghost var oldQueue := Queue;
+      LemmaMapCountEqInterpCount();
+
+      var node := nodemap.Get(x);
+      if node.Some? {
+        var prev := node.value.prev;
+        var next := node.value.next;
+
+        ghost var j := lemmaGetRemoveQueueIndex(Queue, x);
+        if (j > 0) {
+          assert oldContents[x].prev == oldContents[Queue[j-1]];
+        }
+        if (j < |Queue| - 1) {
+          assert oldContents[x].next == oldContents[Queue[j+1]];
+        }
+
+        if (next != null) {
+          if (prev == null) {
+            head_node := next;
+          } else {
+            prev.next := next;
+          }
+
+          next.prev := prev;
+
+          node.value.prev := tail_node;
+          node.value.next := null;
+          if (tail_node != null) {
+            tail_node.next := node.value;
+          } else {
+            head_node := node.value;
+          }
+          tail_node := node.value;
+
+          Repr := {this} + nodemap.Repr + nodemap.Contents.Values;
+          Queue := LruModel.Remove(Queue, x) + [x];
+
+          forall i | 0 <= i < |Queue| - 1
+          ensures nodemap.Contents[Queue[i]].next == nodemap.Contents[Queue[i+1]]
+          {
+            if i == |Queue| - 2 {
+              assert nodemap.Contents[Queue[i]].next == nodemap.Contents[Queue[i+1]];
+            } else if i == j-1 {
+              assert nodemap.Contents[Queue[i]].next == nodemap.Contents[Queue[i+1]];
+            } else if i < j-1 {
+              assert nodemap.Contents[Queue[i]].next == nodemap.Contents[Queue[i+1]];
+            } else {
+              assert nodemap.Contents[Queue[i]].next == nodemap.Contents[Queue[i+1]];
+            }
+          }
+        } else {
+          Repr := {this} + nodemap.Repr + nodemap.Contents.Values;
+          Queue := LruModel.Remove(Queue, x) + [x];
+        }
+      } else {
+        lemmaRemoveNonPresentKeyFromQueue(Queue, x);
+
+        var newnode := new Node(tail_node, null, x);
+        assert newnode.next == null;
+        if (tail_node != null) {
+          tail_node.next := newnode;
+        } else {
+          head_node := newnode;
+        }
+        tail_node := newnode;
+
+        var _ := nodemap.Insert(x, newnode);
+
+        Repr := {this} + nodemap.Repr + nodemap.Contents.Values;
+        Queue := oldQueue + [x];
+
+        assert Queue[|Queue| - 1] == x;
+        assert nodemap.Contents[x] == newnode;
+        assert newnode.next == null;
+        assert nodemap.Contents[Queue[|Queue| - 1]].next == null;
+        forall ref | ref in nodemap.Contents ensures nodemap.Contents[ref].value == ref
+        {
+        }
+        forall i | 0 <= i < |Queue| ensures Queue[i] in nodemap.Contents
+        {
+          if (i == |Queue| - 1) {
+          } else {
+          }
+        }
+      }
+    }
+
+    method Next()
+    returns (x: uint64)
+    requires |I(Queue)| > 0
+    requires Inv()
+    ensures x == LruModel.Next(Queue)
+    {
+      LemmaQueueCountEqInterpCount(Queue);
+      assert head_node != null;
+      x := head_node.value;
+    }
+  }
 }
